Update Zulib

src/Zulib/fsharp/Realized/FStar.UInt32.fs
@@ -1,5 +1,8 @@
 module FStar.UInt32
 
+module Checked = FSharp.Core.Operators.Checked
+open FStar.Pervasives.Native
+
 type uint32 = System.UInt32
 type t = uint32
 type t' = t
@@ -13,14 +16,18 @@ let ones = 4294967295u
 
 let add (a:uint32) (b:uint32) : uint32 = a + b
 let add_mod a b = (add a b) &&& 4294967295u
+let checked_add a b : option<uint32> = try Some (Checked.(+) a b) with | _ -> None
 
 let sub (a:uint32) (b:uint32) : uint32 = a - b
 let sub_mod a b = (sub a b) &&& 4294967295u
+let checked_sub a b : option<uint32> = try Some (Checked.(-) a b) with | _ -> None
 
 let mul (a:uint32) (b:uint32) : uint32 = a * b
 let mul_mod a b = (mul a b) &&& 4294967295u
+let checked_mul a b : option<uint32> = try Some (Checked.(*) a b) with | _ -> None
 
 let div (a:uint32) (b:uint32) : uint32 = a / b
+let checked_div a b : option<uint32> = try Some (a / b) with | _ -> None
 
 let rem (a:uint32) (b:uint32) : uint32 = a % b
 
@@ -41,11 +48,15 @@ let lte (a:uint32) (b:uint32) : bool =  a <= b
 
 let op_Plus_Hat = add
 let op_Plus_Percent_Hat = add_mod
+let op_Plus_Question_Hat = checked_add
 let op_Subtraction_Hat = sub
 let op_Subtraction_Percent_Hat = sub_mod
+let op_Subtraction_Question_Hat = checked_sub
 let op_Star_Hat = mul
 let op_Star_Percent_Hat = mul_mod
+let op_Star_Question_Hat = checked_mul
 let op_Slash_Hat = div
+let op_Slash_Question_Hat = checked_div
 let op_Percent_Hat = rem
 let op_Equals_Hat = eq
 let op_Greater_Hat = gt
@@ -53,6 +64,5 @@ let op_Greater_Equals_Hat = gte
 let op_Less_Hat = lt
 let op_Less_Equals_Hat = lte
 
-let of_string s = uint32.Parse s
 let to_string s = s.ToString()
-//let to_int s = s
+let of_string s : uint32 = uint32.Parse s
