src/Zulib/fsharp/Realized/Zen.Util.fs
@@ -1,0 +1,8 @@
+module Zen.Util
+
+(* TODO: add cost, array's size? *)
+let hashFromBase64 = System.Convert.FromBase64String
+
+let debug x =
+    printfn "%A" x
+    x
