src/Zulib/fstar/Zen.Crypto.fsti
@@ -10,35 +10,35 @@ module U8 = FStar.UInt8
   An explanation of how the costs of crypto primitives was chosen is in `Crypto Analysis.nb`
 *)
 
-type hash      = A.t U8.byte 32
-type signature = A.t U8.byte 64
-type key       = A.t U8.byte 64
+type hash      = Zen.Types.hash
+type signature = Zen.Types.signature
+type key       = Zen.Types.key
 
 val sha2_256: #n:nat
-  -> A.t U8.byte n
+  -> msg: A.t U8.byte n
   -> cost (A.t U8.byte n) M.(n*2 + 160)
 
 val sha2_512: #n:nat
-  -> A.t U8.byte n
+  -> msg: A.t U8.byte n
   -> cost (A.t U8.byte n) M.(n*7 + 710)
 
 val sha3_256: #n:nat
-  -> A.t U8.byte n
+  -> msg: A.t U8.byte n
   -> cost (A.t U8.byte n) M.(n*6 + 1050)
 
 val sha3_512: #n:nat
-  -> A.t U8.byte n
+  -> msg: A.t U8.byte n
   -> cost (A.t U8.byte n) M.(n*8 + 800)
 
 val sign: #n:nat
   -> msg: A.t U8.byte n
-  -> key: A.t U8.byte 64
-  -> A.t U8.byte 64
+  -> key
+  -> signature
 
 val verify: #n:nat
   -> msg: A.t U8.byte n
-  -> signature: A.t U8.byte 64
-  -> key: A.t U8.byte 64
+  -> signature
+  -> pubkey: key
   -> bool
 (*
 (** verifies a signature on an instruction and data for a particular contract. *)
@@ -50,3 +50,4 @@ val verifyCommand: #n:nat
   -> key: A.t U8.byte 64
   -> bool
 *)
+val verifyInputMsg: Zen.Types.inputMsg -> key -> bool
