src/Zulib/fstar/Zen.Types.Extracted.fst
@@ -6,7 +6,6 @@ module     U8 = FStar.UInt8
 module    U32 = FStar.UInt32
 module    U64 = FStar.UInt64
 module Realized = Zen.Types.Realized
-module Crypto = Zen.Crypto
 
 type lockCore = Realized.lockCore
 type contract = Realized.contract
@@ -15,7 +14,9 @@ type extraData = Realized.extraData
 
 type byte = U8.byte
 type opcode = U8.t
-type hash : eqtype = Zen.Crypto.hash
+type hash      = A.t U8.byte 32
+type signature = A.t U8.byte 64
+type key       = A.t U8.byte 64
 type spend = {asset: hash; amount: U64.t}
 type outpoint = {txHash: hash; index: U32.t}
 type witness (n:nat) = A.t byte n
@@ -39,11 +40,11 @@ noeq type data : nat -> Type =
   | Byte: v:U8.t -> data 1
   | Empty: data 0
   | Hash: v:hash -> data 1
-  | Key: v:Crypto.key -> data 1
+  | Key: v:key -> data 1
   | Outpoint: v:outpoint -> data 1
   | Output: v:output -> data 1
   | OutputLock: v:outputLock -> data 1
-  | Sig: v:Crypto.signature -> data 1
+  | Sig: v:signature -> data 1
   | UInt8 : v:U8.t -> data 1
   | UInt32: v:U32.t -> data 1
   | UInt64: v:U64.t -> data 1
@@ -53,10 +54,10 @@ noeq type data : nat -> Type =
   | ByteArray:  l:nat -> a: A.t U8.t l -> data l
   | HashVector: l:nat -> v: V.t hash l -> data l
   | HashArray:  l:nat -> a: A.t hash l -> data l
-  | KeyVector: l:nat -> v: V.t Crypto.key l -> data l
-  | KeyArray:  l:nat -> a: A.t Crypto.key l -> data l
-  | SigVector: l:nat -> v: V.t Crypto.signature l -> data l
-  | SigArray:  l:nat -> a: A.t Crypto.signature l -> data l
+  | KeyVector: l:nat -> v: V.t key l -> data l
+  | KeyArray:  l:nat -> a: A.t key l -> data l
+  | SigVector: l:nat -> v: V.t signature l -> data l
+  | SigArray:  l:nat -> a: A.t signature l -> data l
   | OutpointVector: l:nat -> v: V.t outpoint l -> data l
   | OutpointArray:  l:nat -> a: A.t outpoint l -> data l
   | OutputVector: l:nat -> v: V.t output l -> data l
@@ -69,6 +70,7 @@ noeq type data : nat -> Type =
   | UInt32Array:  l:nat -> a: A.t U32.t l -> data l
   | UInt64Vector: l:nat -> v: V.t U64.t l -> data l
   | UInt64Array:  l:nat -> a: A.t U64.t l -> data l
+  | Optional: l:nat -> option (data l) -> data (l+1)
   | Data2: n1:nat -> n2:nat -> _1:data n1 -> _2:data n2 -> data (n1+n2)
   | Data3: n1:nat -> n2:nat -> n3:nat -> _1:data n1 -> _2:data n2 -> _3:data n3 -> data (n1+n2+n3)
   | Data4: n1:nat -> n2:nat -> n3:nat -> n4:nat -> _1:data n1 -> _2:data n2 -> _3:data n3 -> _4:data n4 -> data (n1+n2+n3+n4)
@@ -93,12 +95,11 @@ and outputLock =
   | ContractLock: contractHash:hash -> n:nat -> data n -> outputLock
   | HighVLock: lockcore:lockCore -> typeCode:nat -> outputLock
 and output = {lock: outputLock; spend: spend}
-(*)
 type inputData (n:nat) = data n
 
-unopteq type transactionSkeleton = | Tx: l1:nat -> outpoints:V.t outpoint l1
-                                      -> l2:nat -> outputs:  V.t output l2
-                                      -> l3:nat -> data:data l3
+unopteq type transactionSkeleton = | Tx: #l1:nat -> outpoints:V.t outpoint l1
+                                      -> #l2:nat -> outputs:  V.t output l2
+                                      -> option (l3:nat & data l3)
                                       -> transactionSkeleton
 
 type utxo = outpoint -> option output
@@ -107,10 +108,19 @@ unopteq type inputMsg = {
   cmd: opcode;
   data: n:nat & inputData n;
   contractHash: hash;
-  utxo: utxo;
-  lastTx: option outpoint
-  }
+  utxo: utxo
+}
 
+
+val maxCost: nat
+let maxCost = 200
+
+noeq type costFunction = | CostFunc: #n:nat{n<=maxCost} -> f:(inputMsg -> Zen.Cost.t nat n) -> costFunction
+
+noeq type mainFunction =
+  | MainFunc: cf:costFunction
+           -> mf:(imsg:inputMsg -> Zen.Cost.t (result transactionSkeleton) (Zen.Cost.force ((CostFunc?.f cf) imsg)))
+           -> mainFunction
 
 //val contractVersion : extendedContract -> U32.t
 
