src/Zulib/fstar/Zen.Merkle.fsti
@@ -1,0 +1,20 @@
+module Zen.Merkle
+
+open Zen.Cost
+module A = Zen.Array
+module M = FStar.Mul
+module C = Zen.Crypto
+module U32 = FStar.UInt32
+open Zen.Types.Extracted
+
+
+val rootFromAuditPath: #n:nat
+  -> C.hash
+  -> U32.t
+  -> A.t C.hash n
+  -> cost (C.hash) n
+
+val hashData: #n:nat
+-> data n
+-> cost (option hash) M.(n*384 + 1050)
+    
