src/Zulib/fstar/Zen.Util.fsti
@@ -1,0 +1,12 @@
+module Zen.Util
+
+open Zen.Types.Extracted
+
+module  C = Zen.Crypto
+module  A = Zen.Array
+module U8 = FStar.UInt8
+
+(* TODO: add cost; array's size?; handle exceptions using option *)
+val hashFromBase64: string -> A.t U8.byte 32
+
+val debug : 'a -> 'a
