src/Zulib/fstar/Zen.Wallet.fsti
@@ -1,0 +1,54 @@
+module Zen.Wallet
+
+open Zen.Base
+open Zen.Cost
+open Zen.Types
+open FStar.UInt64
+
+module V = Zen.Vector
+
+assume new type wallet
+assume Wallet_Eq: hasEq wallet
+
+val getTransaction: wallet -> transactionSkeleton
+
+val getFunds: wallet -> (asset:hash) -> UInt64.t
+
+val getFundsFrom: wallet -> (pkhash:hash) -> (asset:hash) -> UInt64.t
+
+assume GetFundsFrom_GetFunds:
+  forall (w:wallet) (asset:hash) (pkhash:hash).
+  getFundsFrom w pkhash asset <=^ w `getFunds` asset
+
+val addOutput: w:wallet
+  -> o: output{o.spend.amount <=^ w `getFunds` o.spend.asset}
+  -> wallet
+
+(* If a wallet can spend an output o with amount m of asset a, then spending o:
+  1) Increases the length of the transactionSkeleton outputs by 1
+  2) Results in the last transactionSkeleton output being equal to o *)
+assume AddOutput_GetTransaction:
+  forall (w:wallet) (o:output{o.spend.amount <=^ w `getFunds` o.spend.asset}).
+  let num_outputs = Tx?.l2 @ getTransaction w in
+  match getTransaction (addOutput w o) with
+  | Tx #_ _ #l outputs _ ->
+    l = num_outputs + 1 /\ force (V.nth outputs (l-1)) == o
+
+(*
+  If a wallet can spend an output o with amount m of asset a, then spending o:
+  1) Reduces the amount of asset a in the wallet by m
+*)
+assume AddOutput_getFunds:
+  forall (w:wallet) (o:output{o.spend.amount <=^ w `getFunds` o.spend.asset}).
+  getFunds (w `addOutput` o) o.spend.asset = getFunds w o.spend.asset -^ o.spend.amount
+
+val getOwner: wallet -> owner:hash
+
+(*
+  If a wallet can spend an output o with amount m of asset a, then spending o:
+  1) Increases the length of the transactionSkeleton outputs by 1
+  2) Results in the last transactionSkeleton output being equal to o
+*)
+assume AddOutput_getOwner:
+  forall w (o:output{o.spend.amount <=^ w `getFunds` o.spend.asset}).
+  getOwner (w `addOutput` o) = getOwner w
