src/Zulib/build.sh
@@ -1,0 +1,11 @@
+#!/bin/sh
+
+mono ../../.paket/paket.exe restore
+
+exit_code=$?
+  if [ $exit_code -ne 0 ]; then
+    exit $exit_code
+  fi
+
+ulimit -n 2000
+mono ../../packages/FAKE/tools/FAKE.exe $@ --fsiargs -d:MONO build.fsx
